cub module renaming

coq/lib/P4cub/Semantics/Dynamic/BigStep/Interpreter.v
@@ -11,23 +11,16 @@ From Poulet4 Require Import
   P4light.Architecture.Target
   Utils.Util.ListUtil.
 
-Import
-  Option
-  Val.ValueNotations
-  ExprNotations
-  ParserNotations
-  Val.LValueNotations
-  StmtNotations
-  String.
+Import Option String.
 
 Local Open Scope type_scope.
 
-Section Expr.
+Section Exp.
 
   (** Binds variables' de Bruijn indices to their values *)
-  Variable ϵ : list Val.v.
+  Variable ϵ : list Val.t.
 
-  Definition to_bit (v : Val.v) : option (N * Z) :=
+  Definition to_bit (v : Val.t) : option (N * Z) :=
     match v with
     | Val.Bit w n => Some (w, n)
     | _ => None
@@ -41,247 +34,247 @@ Section Expr.
 
   Definition interpret_index array n := index (Z.to_nat n) array.
 
-  (** [interpret_expr e] is [Some v] iff [⟨ ϵ, e ⟩ ⇓ v], or [None] if [e] is
+  (** [interpret_exp e] is [Some v] iff [⟨ ϵ, e ⟩ ⇓ v], or [None] if [e] is
       ill-typed *)
-  Fixpoint interpret_expr (e : Expr.e) : option Val.v :=
+  Fixpoint interpret_exp (e : Exp.t) : option Val.t :=
     match e with
-    | Expr.Bool b => mret $ Val.Bool b
-    | Expr.Bit w n => mret $ Val.Bit w n
-    | Expr.Int w n => mret $ Val.Int w n
-    | Expr.Var _ _ index => nth_error ϵ index
-    | Expr.VarBit m w n => mret $ Val.VarBit m w n
-    | Expr.Slice hi lo e => slice_val hi lo =<< interpret_expr e
-    | Expr.Cast t e => eval_cast t =<< interpret_expr e
-    | Expr.Uop _ op e => eval_uop op =<< interpret_expr e
-    | Expr.Bop _ op e1 e2 =>
-      let* v1 := interpret_expr e1 in
-      let* v2 := interpret_expr e2 in
-      eval_bop op v1 v2
-    | Expr.Lists ls es => map_monad interpret_expr es >>| Val.Lists ls
-    | Expr.Index _ array index =>
-      let* array := interpret_expr array in
-      let* (_, index) := to_bit =<< interpret_expr index in
+    | Exp.Bool b => mret $ Val.Bool b
+    | Exp.Bit w n => mret $ Val.Bit w n
+    | Exp.Int w n => mret $ Val.Int w n
+    | Exp.Var _ _ index => nth_error ϵ index
+    | Exp.VarBit m w n => mret $ Val.VarBit m w n
+    | Exp.Slice hi lo e => slice_val hi lo =<< interpret_exp e
+    | Exp.Cast t e => eval_cast t =<< interpret_exp e
+    | Exp.Uop _ op e => eval_una op =<< interpret_exp e
+    | Exp.Bop _ op e1 e2 =>
+      let* v1 := interpret_exp e1 in
+      let* v2 := interpret_exp e2 in
+      eval_bin op v1 v2
+    | Exp.Lists ls es => map_monad interpret_exp es >>| Val.Lists ls
+    | Exp.Index _ array index =>
+      let* array := interpret_exp array in
+      let* (_, index) := to_bit =<< interpret_exp index in
       interpret_index array index
-    | Expr.Member _ field member => index field =<< interpret_expr member
-    | Expr.Error err => mret $ Val.Error err
+    | Exp.Member _ field member => index field =<< interpret_exp member
+    | Exp.Error err => mret $ Val.Error err
     end.
 
-  Theorem interpret_expr_sound : 
-    forall e v, interpret_expr e = Some v -> ⟨ ϵ, e ⟩ ⇓ v.
+  Theorem interpret_exp_sound : 
+    forall e v, interpret_exp e = Some v -> ⟨ ϵ, e ⟩ ⇓ v.
   Proof.
-    induction e using custom_e_ind.
+    induction e using custom_exp_ind.
     - intros. inv H. constructor.
     - intros. inv H. constructor.
     - intros. inv H. constructor.
     - intros. inv H. constructor.
     - intros. inv H. constructor. assumption.
     - simpl. unfold option_bind. intros.
-      destruct (interpret_expr e); try discriminate.
+      destruct (interpret_exp e); try discriminate.
       econstructor; eauto.
     - simpl. unfold option_bind. intros.
-      destruct (interpret_expr e); try discriminate.
+      destruct (interpret_exp e); try discriminate.
       econstructor; eauto.
     - simpl. unfold option_bind. intros.
-      destruct (interpret_expr e); try discriminate.
+      destruct (interpret_exp e); try discriminate.
       econstructor; eauto.
     - simpl. unfold option_bind. intros.
-      destruct (interpret_expr e1); try discriminate.
-      destruct (interpret_expr e2); try discriminate.
+      destruct (interpret_exp e1); try discriminate.
+      destruct (interpret_exp e2); try discriminate.
       econstructor; eauto.
     - simpl. unfold option_bind, map_monad, "∘". intros.
-      destruct (sequence (map interpret_expr exps)) eqn:E; try discriminate.
+      destruct (sequence (map interpret_exp es)) eqn:E; try discriminate.
       inv H0.
       apply sequence_Forall2 in E.
       apply Forall2_map_comm_fwd in E.
       constructor. generalize dependent l0.
-      induction exps; intros; inv H; inv E; constructor; auto.
+      induction es; intros; inv H; inv E; constructor; auto.
     - simpl. unfold option_bind, interpret_index, index, to_bit. intros.
-      destruct (interpret_expr e1);
-      destruct (interpret_expr e2);
+      destruct (interpret_exp e1);
+      destruct (interpret_exp e2);
       try discriminate.
-      destruct v1; destruct v0; try discriminate.
+      destruct t; destruct t0; try discriminate.
       econstructor; eauto.
     - simpl. unfold option_bind, index. intros.
-      destruct (interpret_expr e); try discriminate.
-      destruct v0; try discriminate.
+      destruct (interpret_exp e); try discriminate.
+      destruct t; try discriminate.
       econstructor; eauto.
-    - intros. inv H. constructor.
+    - intros. unravel in *. inv H. constructor.
     Qed.
 
-    Theorem interpret_expr_complete :
-      forall e v, ⟨ ϵ, e ⟩ ⇓ v -> interpret_expr e = Some v.
+    Theorem interpret_exp_complete :
+      forall e v, ⟨ ϵ, e ⟩ ⇓ v -> interpret_exp e = Some v.
     Proof.
-      induction e using custom_e_ind.
+      induction e using custom_exp_ind.
       - intros. inv H. reflexivity.
       - intros. inv H. reflexivity.
       - intros. inv H. reflexivity.
       - intros. inv H. reflexivity.
       - intros. inv H. assumption.
       - intros. inv H. simpl. unfold option_bind.
-        destruct (interpret_expr e); apply IHe in H5; try discriminate.
+        destruct (interpret_exp e); apply IHe in H5; try discriminate.
         inv H5. assumption.
       - intros. inv H. simpl. unfold option_bind.
-        destruct (interpret_expr e); apply IHe in H4; try discriminate.
+        destruct (interpret_exp e); apply IHe in H4; try discriminate.
         inv H4. assumption.
       - intros. inv H. simpl. unfold option_bind.
-        destruct (interpret_expr e); apply IHe in H5; try discriminate.
+        destruct (interpret_exp e); apply IHe in H5; try discriminate.
         inv H5. assumption.
       - intros. inv H. simpl. unfold option_bind.
-        destruct (interpret_expr e1); apply IHe1 in H6;
-        destruct (interpret_expr e2); apply IHe2 in H7;
+        destruct (interpret_exp e1); apply IHe1 in H6;
+        destruct (interpret_exp e2); apply IHe2 in H7;
         try discriminate. inv H6. inv H7. assumption.
       - intros. simpl. unfold option_bind, map_monad, "∘".
-        inv H0. destruct (sequence (map interpret_expr exps)) eqn:E.
+        inv H0. destruct (sequence (map interpret_exp es)) eqn:E.
         + apply sequence_Forall2 in E.
           apply Forall2_map_comm_fwd in E.
           repeat f_equal.
           generalize dependent vs.
           generalize dependent l0.
-          induction exps; intros;
+          induction es; intros;
           inv E; inv H; inv H4; auto.
           apply H3 in H1. assert (Some y0 = Some y).
           { rewrite <- H1. rewrite H2. reflexivity. }
           inv H. f_equal. auto.
-        + assert (sequence (map interpret_expr exps) <> Some vs).
+        + assert (sequence (map interpret_exp es) <> Some vs).
           { rewrite E. discriminate. }
           clear E.
-          apply (contra_not (Forall2_sequence (map interpret_expr exps) vs)) in H0.
+          apply (contra_not (Forall2_sequence (map interpret_exp es) vs)) in H0.
           exfalso. apply H0. clear H0. apply Forall2_map_comm_rev.
-          generalize dependent vs. induction exps; intros;
+          generalize dependent vs. induction es; intros;
           inv H4; constructor. inv H; auto. inv H.
-          apply IHexps with (vs := l') in H4; assumption.
+          apply IHes with (vs := l') in H4; assumption.
       - intros. inv H. simpl. unfold option_bind.
-        destruct (interpret_expr e1); apply IHe1 in H5; try discriminate.
-        destruct (interpret_expr e2); apply IHe2 in H6; try discriminate.
+        destruct (interpret_exp e1); apply IHe1 in H5; try discriminate.
+        destruct (interpret_exp e2); apply IHe2 in H6; try discriminate.
         inv H5. inv H6. simpl. assumption.
       - intros. inv H. simpl. unfold option_bind.
-        destruct (interpret_expr e); apply IHe in H5; try discriminate.
+        destruct (interpret_exp e); apply IHe in H5; try discriminate.
         inv H5. simpl. assumption.
       - intros. inv H. reflexivity.
     Qed.
 
-    Lemma interpret_expr_adequate :
-      forall e v, interpret_expr e = Some v <-> ⟨ ϵ, e ⟩ ⇓ v.
+    Lemma interpret_exp_adequate :
+      forall e v, interpret_exp e = Some v <-> ⟨ ϵ, e ⟩ ⇓ v.
     Proof.
       split.
-      - apply interpret_expr_sound.
-      - apply interpret_expr_complete.
+      - apply interpret_exp_sound.
+      - apply interpret_exp_complete.
     Qed.
 
-    Fixpoint interpret_lexpr (e : Expr.e) : option Val.lv :=
+    Fixpoint interpret_lexp (e : Exp.t) : option Lval.t :=
       match e with
-      | Expr.Var _ _ x => mret $ Val.Var x
-      | Expr.Slice hi lo e => interpret_lexpr e >>| Val.Slice hi lo
-      | Expr.Member _ x e => interpret_lexpr e >>| Val.Member x
-      | Expr.Index _ e1 e2 =>
-        let* lv := interpret_lexpr e1 in
-        let^ (_, n) := to_bit =<< interpret_expr e2 in
-        Val.Index (Z.to_N n) lv
+      | Exp.Var _ _ x => mret $ Lval.Var x
+      | Exp.Slice hi lo e => interpret_lexp e >>| Lval.Slice hi lo
+      | Exp.Member _ x e => interpret_lexp e >>| Lval.Member x
+      | Exp.Index _ e1 e2 =>
+        let* lv := interpret_lexp e1 in
+        let^ (_, n) := to_bit =<< interpret_exp e2 in
+        Lval.Index (Z.to_N n) lv
       | _ => None
       end.
 
-    Lemma interpret_lexpr_sound :
-      forall e lv, interpret_lexpr e = Some lv -> l⟨ ϵ , e ⟩ ⇓ lv.
+    Lemma interpret_lexp_sound :
+      forall e lv, interpret_lexp e = Some lv -> l⟨ ϵ , e ⟩ ⇓ lv.
     Proof.
       induction e; try discriminate; intros; inv H; unfold option_bind in *.
       - constructor.
-      - destruct (interpret_lexpr e) eqn:?; try discriminate. inv H1.
+      - destruct (interpret_lexp e) eqn:?; try discriminate. inv H1.
         constructor. auto.
       - unfold to_bit in *.
-        destruct (interpret_lexpr e1); try discriminate.
-        destruct (interpret_expr e2) eqn:?; try discriminate.
-        destruct v; try discriminate.
+        destruct (interpret_lexp e1); try discriminate.
+        destruct (interpret_exp e2) eqn:?; try discriminate.
+        destruct t0; try discriminate.
         inv H1. econstructor; eauto. 
-        apply interpret_expr_sound. eauto.
-      - destruct (interpret_lexpr e); try discriminate.
+        apply interpret_exp_sound. eauto.
+      - destruct (interpret_lexp e); try discriminate.
         inv H1. constructor. auto.
     Qed.
 
-    Lemma interpret_lexpr_complete :
-      forall e lv, l⟨ ϵ , e ⟩ ⇓ lv -> interpret_lexpr e = Some lv.
+    Lemma interpret_lexp_complete :
+      forall e lv, l⟨ ϵ , e ⟩ ⇓ lv -> interpret_lexp e = Some lv.
     Proof.
       intros. induction H; cbn; unfold option_bind in *.
       - reflexivity.
-      - destruct (interpret_lexpr e); try discriminate.
-        f_equal. inv IHlexpr_big_step. auto.
-      - destruct (interpret_lexpr e); try discriminate.
-        f_equal. inv IHlexpr_big_step. auto.
-      - unfold to_bit. destruct (interpret_lexpr e₁) eqn:?; try discriminate.
-        apply interpret_expr_complete in H.
-        destruct (interpret_expr e₂); try discriminate.
-        destruct v; try discriminate.
-        inv H. inv IHlexpr_big_step. auto.
+      - destruct (interpret_lexp e); try discriminate.
+        f_equal. inv IHlexp_big_step. auto.
+      - destruct (interpret_lexp e); try discriminate.
+        f_equal. inv IHlexp_big_step. auto.
+      - unfold to_bit. destruct (interpret_lexp e₁) eqn:?; try discriminate.
+        apply interpret_exp_complete in H.
+        destruct (interpret_exp e₂); try discriminate.
+        destruct t0; try discriminate.
+        inv H. inv IHlexp_big_step. auto.
     Qed.
 
-    Lemma interpret_lexpr_adequate : forall e lv, 
-      interpret_lexpr e = Some lv <-> l⟨ ϵ , e ⟩ ⇓ lv.
+    Lemma interpret_lexp_adequate : forall e lv, 
+      interpret_lexp e = Some lv <-> l⟨ ϵ , e ⟩ ⇓ lv.
     Proof.
       split.
-      - apply interpret_lexpr_sound.
-      - apply interpret_lexpr_complete.
+      - apply interpret_lexp_sound.
+      - apply interpret_lexp_complete.
     Qed.
 
-    Definition interpret_parser_expr (pat : Parser.pt) : option Parser.state_label :=
+    Definition interpret_parser_exp (pat : Trns.t) : option Lbl.t :=
       match pat with
-      | Parser.Direct st => mret st
-      | Parser.Select e default cases =>
-        let^ v := interpret_expr e in
+      | Trns.Direct st => mret st
+      | Trns.Select e default cases =>
+        let^ v := interpret_exp e in
         match Field.find_value (fun p => match_pattern p v) cases with
         | Some st => st
         | None => default
         end
       end.
 
-    Lemma interpret_parser_expr_sound :
-      forall pat state, interpret_parser_expr pat = Some state -> p⟨ ϵ , pat ⟩ ⇓ state.
+    Lemma interpret_parser_exp_sound :
+      forall pat state, interpret_parser_exp pat = Some state -> p⟨ ϵ , pat ⟩ ⇓ state.
     Proof.
       intros. destruct pat; inv H.
       - constructor.
       - unfold option_bind in *.
-        destruct (interpret_expr discriminee) eqn:?; try discriminate.
-        inv H1. constructor. apply interpret_expr_sound. assumption.
+        destruct (interpret_exp discriminee) eqn:?; try discriminate.
+        inv H1. constructor. apply interpret_exp_sound. assumption.
     Qed.
 
-    Lemma interpret_parser_expr_complete :
-      forall pat state, p⟨ ϵ , pat ⟩ ⇓ state -> interpret_parser_expr pat = Some state.
+    Lemma interpret_parser_exp_complete :
+      forall pat state, p⟨ ϵ , pat ⟩ ⇓ state -> interpret_parser_exp pat = Some state.
     Proof.
       intros. inv H; cbn.
       - reflexivity.
       - unfold option_bind in *.
-        apply interpret_expr_complete in H0.
-        destruct (interpret_expr e) eqn:?; try discriminate.
+        apply interpret_exp_complete in H0.
+        destruct (interpret_exp e) eqn:?; try discriminate.
         inv H0. reflexivity. 
     Qed.
 
-    Lemma interpret_parser_expr_adequate :
-      forall pat state, interpret_parser_expr pat = Some state <-> p⟨ ϵ , pat ⟩ ⇓ state.
+    Lemma interpret_parser_exp_adequate :
+      forall pat state, interpret_parser_exp pat = Some state <-> p⟨ ϵ , pat ⟩ ⇓ state.
     Proof.
       split.
-      - apply interpret_parser_expr_sound.
-      - apply interpret_parser_expr_complete.
+      - apply interpret_parser_exp_sound.
+      - apply interpret_parser_exp_complete.
     Qed.
 
-End Expr.
+End Exp.
 
-Section Parser.
+Section Trns.
 
-  Variable ϵ : list Val.v.
+  Variable ϵ : list Val.t.
 
   Open Scope pat_scope.
 
-  Definition interpret_pre_match (e : @MatchPreT unit) : option Parser.pat :=
+  Definition interpret_pre_match (e : @MatchPreT unit) : option Pat.t :=
     match e with
-    | MatchDontCare => mret $ Parser.Wild
+    | MatchDontCare => mret $ Pat.Wild
     | MatchMask l1 l2 =>
-        let* (w1, n1) := to_bit =<< interpret_expr [] =<< unembed_expr l1 in
-        let* (w2, n2) := to_bit =<< interpret_expr [] =<< unembed_expr l2 in
+        let* (w1, n1) := to_bit =<< interpret_exp [] =<< unembed_exp l1 in
+        let* (w2, n2) := to_bit =<< interpret_exp [] =<< unembed_exp l2 in
         guard (N.eqb w1 w2) ;;
-        mret $ Parser.Mask (w1 PW n1) (w2 PW n2)
+        mret $ Pat.Mask (w1 PW n1) (w2 PW n2)
     | MatchRange l1 l2 =>
-        let* (w1, n1) := to_bit =<< interpret_expr [] =<< unembed_expr l1 in
-        let* (w2, n2) := to_bit =<< interpret_expr [] =<< unembed_expr l2 in
+        let* (w1, n1) := to_bit =<< interpret_exp [] =<< unembed_exp l1 in
+        let* (w2, n2) := to_bit =<< interpret_exp [] =<< unembed_exp l2 in
         guard (N.eqb w1 w2) ;;
-        mret $ Parser.Range (w1 PW n1) (w2 PW n2)
+        mret $ Pat.Range (w1 PW n1) (w2 PW n2)
     | _ => None
     end.
-End Parser.
+End Trns.
