coq/lib/P4cub/Semantics/Dynamic/BigStep/Typing.v
@@ -5,63 +5,62 @@ From Poulet4.P4cub.Semantics Require Import Static.Static
      Dynamic.BigStep.Value.Value
      Dynamic.BigStep.Semantics
      Dynamic.BigStep.TypeSoundness.
-Import AllCubNotations Val.ValueNotations Val.LValueNotations.
 
-(** An expression [e] evaluates in a "well-typed" way.
+(** An expession [e] evaluates in a "well-typed" way.
     Progress & preservation included all in one. *)
-Definition semantic_expr_typing
-  (Δ : nat) (Γ : list Expr.t) (e: Expr.e) (τ : Expr.t) : Prop :=
-  forall ϵ : list Val.v,
-    Forall2 type_value ϵ Γ ->
-    (exists v : Val.v, ⟨ ϵ, e ⟩ ⇓ v) /\
-      (forall v : Val.v, ⟨ ϵ, e ⟩ ⇓ v -> ⊢ᵥ v ∈ τ).
+Definition semantic_exp_typing
+  (Δ : nat) (Γ : list Typ.t) (e: Exp.t) (τ : Typ.t) : Prop :=
+  forall ϵ : list Val.t,
+    Forall2 type_val ϵ Γ ->
+    (exists v : Val.t, ⟨ ϵ, e ⟩ ⇓ v) /\
+      (forall v : Val.t, ⟨ ϵ, e ⟩ ⇓ v -> ⊢ᵥ v ∈ τ).
 
 Notation "⟪ Δ , Γ ⟫ ⊢ e ∈ τ"
-  := (semantic_expr_typing Δ Γ e τ)
+  := (semantic_exp_typing Δ Γ e τ)
        (at level 80, no associativity) : type_scope.
 
-Ltac unfold_sem_typ_expr_goal :=
+Ltac unfold_sem_typ_exp_goal :=
   match goal with
   | |- ⟪ _ , _ ⟫ ⊢ _ ∈ _
-    => unfold semantic_expr_typing;
+    => unfold semantic_exp_typing;
       intros ϵ henv; split;
       [| intros v Hv; inv Hv]
   end.
 
-Ltac unfold_sem_typ_expr_hyp :=
+Ltac unfold_sem_typ_exp_hyp :=
   match goal with
   | H: ⟪ _ , _ ⟫ ⊢ _ ∈ _
-    |- _ => unfold semantic_expr_typing in H
+    |- _ => unfold semantic_exp_typing in H
   end.
 
-Ltac unfold_sem_typ_expr :=
-  repeat unfold_sem_typ_expr_hyp;
-  unfold_sem_typ_expr_goal.
+Ltac unfold_sem_typ_exp :=
+  repeat unfold_sem_typ_exp_hyp;
+  unfold_sem_typ_exp_goal.
 
 (** Typing Derivations. *)
 Section Rules.
   Variable Δ : nat.
-  Variable Γ : list Expr.t.
+  Variable Γ : list Typ.t.
 
-  Local Hint Constructors expr_big_step : core.
-  Local Hint Constructors type_value : core.
+  Local Hint Constructors exp_big_step : core.
+  Local Hint Constructors type_val : core.
   
   Lemma sem_typ_bool : forall b : bool,
-      ⟪ Δ , Γ ⟫ ⊢ b ∈ Expr.TBool.
+      ⟪ Δ , Γ ⟫ ⊢ Exp.Bool b ∈ Typ.Bool.
   Proof.
-    intros b; unfold_sem_typ_expr; eauto.
+    intros b; unfold_sem_typ_exp; eauto.
   Qed.
   
   Lemma sem_typ_uop : forall op τ τ' e,
-      uop_type op τ τ' ->
+      una_type op τ τ' ->
       ⟪ Δ , Γ ⟫ ⊢ e ∈ τ ->
-      ⟪ Δ , Γ ⟫ ⊢ Expr.Uop τ' op e ∈ τ'.
+      ⟪ Δ , Γ ⟫ ⊢ Exp.Uop τ' op e ∈ τ'.
   Proof.
-    intros op t t' e Huop He; unfold_sem_typ_expr.
+    intros op t t' e Huna He; unfold_sem_typ_exp.
   Abort.
 
-  Local Hint Resolve expr_big_step_preservation : core.
-  Local Hint Resolve expr_big_step_progress : core.
+  Local Hint Resolve exp_big_step_preservation : core.
+  Local Hint Resolve exp_big_step_progress : core.
   
   Lemma soundness : forall e τ,
       `⟨ Δ , Γ ⟩ ⊢ e ∈ τ -> ⟪ Δ , Γ ⟫ ⊢ e ∈ τ.
@@ -70,13 +69,13 @@ Section Rules.
       destruct H as (? & ?); eauto.
   Qed.
 
-  Local Hint Constructors type_expr : core.
+  Local Hint Constructors type_exp : core.
   
   Lemma completeness : forall e τ,
       ⟪ Δ , Γ ⟫ ⊢ e ∈ τ -> `⟨ Δ, Γ ⟩ ⊢ e ∈ τ.
   Proof.
-    intro e; induction e using custom_e_ind;
-      intros t Hsem; unfold_sem_typ_expr_hyp.
+    intro e; induction e using custom_exp_ind;
+      intros t Hsem; unfold_sem_typ_exp_hyp.
     - (* hmmmm... *)
   Abort.
 End Rules.
