coq/lib/P4cub/Semantics/Dynamic/SmallStep/Semantics.v
@@ -7,7 +7,7 @@ Import String.
 (* TODO: correctly handle type parameters/arguments. *)
 
 Module Step.
-  Import AllCubNotations Clmt.Notations.
+  Import Clmt.Notations.
   Open Scope climate_scope.
 
   (** Continuation statements. *)
@@ -28,93 +28,93 @@ Module Step.
            (at level 80, no associativity).
   
   (** Expression evaluation. *)
-  Inductive expr_step (ϵ : list Expr.e) : Expr.e -> Expr.e -> Prop :=
+  Inductive exp_step (ϵ : list Exp.t) : Exp.t -> Exp.t -> Prop :=
   | step_var τ og x e :
     nth_error ϵ x = Some e ->
-    ⟨ ϵ, Expr.Var τ og x ⟩ -->  e
+    ⟨ ϵ, Exp.Var τ og x ⟩ -->  e
   | step_slice e e' hi lo :
     ⟨ ϵ, e ⟩ -->  e' ->
-    ⟨ ϵ, Expr.Slice hi lo e ⟩ -->  Expr.Slice hi lo e'
+    ⟨ ϵ, Exp.Slice hi lo e ⟩ -->  Exp.Slice hi lo e'
   | step_slice_eval v v' hi lo :
     eval_slice hi lo v = Some v' ->
     value v ->
-    ⟨ ϵ, Expr.Slice hi lo v ⟩ -->  v'
+    ⟨ ϵ, Exp.Slice hi lo v ⟩ -->  v'
   | step_cast τ e e' :
     ⟨ ϵ, e ⟩ -->  e' ->
-    ⟨ ϵ, Expr.Cast τ e ⟩ -->  Expr.Cast τ e'
+    ⟨ ϵ, Exp.Cast τ e ⟩ -->  Exp.Cast τ e'
   | step_cast_eval τ v v' :
     eval_cast τ v = Some v' ->
     value v ->
-    ⟨ ϵ, Expr.Cast τ v ⟩ -->  v'
+    ⟨ ϵ, Exp.Cast τ v ⟩ -->  v'
   | step_uop τ op e e' :
     ⟨ ϵ, e ⟩ -->  e' ->
-    ⟨ ϵ, Expr.Uop τ op e ⟩ -->  Expr.Uop τ op e'
+    ⟨ ϵ, Exp.Uop τ op e ⟩ -->  Exp.Uop τ op e'
   | step_uop_eval op τ v v' :
-    eval_uop op v = Some v' ->
+    eval_una op v = Some v' ->
     value v ->
-    ⟨ ϵ, Expr.Uop τ op v ⟩ -->  v'
+    ⟨ ϵ, Exp.Uop τ op v ⟩ -->  v'
   | step_bop_l τ op el el' er :
     ⟨ ϵ, el ⟩ -->  el' ->
-    ⟨ ϵ, Expr.Bop τ op el er ⟩ -->  Expr.Bop τ op el' er
+    ⟨ ϵ, Exp.Bop τ op el er ⟩ -->  Exp.Bop τ op el' er
   | step_bop_r τ op vl er er' :
     value vl ->
     ⟨ ϵ, er ⟩ -->  er' ->
-    ⟨ ϵ, Expr.Bop τ op vl er ⟩ -->  Expr.Bop τ op vl er'
+    ⟨ ϵ, Exp.Bop τ op vl er ⟩ -->  Exp.Bop τ op vl er'
   | step_bop_eval τ op v vl vr :
-    eval_bop op vl vr = Some v ->
+    eval_bin op vl vr = Some v ->
     value vl -> value vr ->
-    ⟨ ϵ, Expr.Bop τ op vl vr ⟩ -->  v
+    ⟨ ϵ, Exp.Bop τ op vl vr ⟩ -->  v
   | step_member τ x e e' :
     ⟨ ϵ, e ⟩ -->  e' ->
-    ⟨ ϵ, Expr.Member τ x e ⟩ -->  Expr.Member τ x e
+    ⟨ ϵ, Exp.Member τ x e ⟩ -->  Exp.Member τ x e
   | step_member_eval τ x ls vs v :
     nth_error vs x = Some v ->
     Forall value vs ->
-    ⟨ ϵ, Expr.Member τ x (Expr.Lists ls vs) ⟩ -->  v
+    ⟨ ϵ, Exp.Member τ x (Exp.Lists ls vs) ⟩ -->  v
   | step_index_l τ e₁ e₁' e₂ :
     ⟨ ϵ, e₁ ⟩ --> e₁' ->
-    ⟨ ϵ, Expr.Index τ e₁ e₂ ⟩ --> Expr.Index τ e₁' e₂
+    ⟨ ϵ, Exp.Index τ e₁ e₂ ⟩ --> Exp.Index τ e₁' e₂
   | step_index_r τ v₁ e₂ e₂' :
     value v₁ ->
     ⟨ ϵ, e₂ ⟩ --> e₂' ->
-    ⟨ ϵ, Expr.Index τ v₁ e₂ ⟩ --> Expr.Index τ v₁ e₂'
+    ⟨ ϵ, Exp.Index τ v₁ e₂ ⟩ --> Exp.Index τ v₁ e₂'
   | step_index_eval τ ls vs w n v :
     nth_error vs (Z.to_nat n) = Some v ->
     Forall value vs ->
-    ⟨ ϵ, Expr.Index τ (Expr.Lists ls vs) (w `W n)%expr ⟩ --> v
+    ⟨ ϵ, Exp.Index τ (Exp.Lists ls vs) (w `W n)%exp ⟩ --> v
   | step_lists prefix suffix ls e e' :
     Forall value prefix ->
     ⟨ ϵ, e ⟩ -->  e' ->
-    ⟨ ϵ, Expr.Lists ls (prefix ++ e :: suffix) ⟩
-      -->  Expr.Lists ls (prefix ++ e' :: suffix)
-  where "⟨ ϵ , e1 ⟩ '-->' e2" := (expr_step ϵ e1 e2) : type_scope.
+    ⟨ ϵ, Exp.Lists ls (prefix ++ e :: suffix) ⟩
+      -->  Exp.Lists ls (prefix ++ e' :: suffix)
+  where "⟨ ϵ , e1 ⟩ '-->' e2" := (exp_step ϵ e1 e2) : type_scope.
 
-  (** TODO: add Expr.Index to this. *)
-  Inductive lvalue_step : Expr.e -> Expr.e -> Prop :=
+  (** TODO: add Exp.Index to this. *)
+  Inductive lvalue_step : Exp.t -> Exp.t -> Prop :=
   | lstep_slice e e' hi lo :
     lvalue_step e e' ->
-    lvalue_step (Expr.Slice hi lo e) (Expr.Slice hi lo e')
+    lvalue_step (Exp.Slice hi lo e) (Exp.Slice hi lo e')
   | lstep_member τ x e e' :
     lvalue_step e e' ->
-    lvalue_step (Expr.Member τ x e) (Expr.Member τ x e').
+    lvalue_step (Exp.Member τ x e) (Exp.Member τ x e').
   
   Reserved Notation "'π' envn , pe1 '-->' pe2"
            (at level 80, no associativity).
   
-  Inductive step_parser_expr (ϵ : list Expr.e)
-    : Parser.pt -> Parser.pt -> Prop :=
+  Inductive step_parser_exp (ϵ : list Exp.t)
+    : Trns.t -> Trns.t -> Prop :=
   | step_select_discriminee e e' d cases :
     ⟨ ϵ, e ⟩ -->  e' ->
-    π ϵ, Parser.Select e d cases -->  Parser.Select e' d cases
+    π ϵ, Trns.Select e d cases -->  Trns.Select e' d cases
   | step_select_resolve v d cases :
       value v ->
       let pe := match Field.find_value (fun _ => false) cases with (** TODO!! *)
                 | None => d
                 | Some pe => pe
                 end in
-      π ϵ, Parser.Select v d cases -->  Parser.Direct pe
+      π ϵ, Trns.Select v d cases -->  Trns.Direct pe
   where "'π' envn , pe1 '-->' pe2"
-    := (step_parser_expr envn pe1 pe2).
+    := (step_parser_exp envn pe1 pe2).
 
   (*
   Reserved Notation "'ℸ' cfg , tbls , aa , fns , ins , ϵ1 , k1 '-->' k2 , ϵ2"
@@ -164,20 +164,20 @@ Module Step.
       κ b{ s }b ⋅ k -->  κ s ⋅ ∫ ϵ ⊗ k, ϵ
   | step_kblock (ϵk : eenv) (k : kstmt) :
       ℸ cfg, tbls, aa, fns, ins, ϵ, ∫ ϵk ⊗ k -->  k, (ϵk ≪ ϵ)
-  (*| step_vardecl (τ : Expr.t) (x : string)  (k : kstmt) :
+  (*| step_vardecl (τ : Typ.t) (x : string)  (k : kstmt) :
       let v := edefault i τ in
       ℸ cfg, tbls, aa, fns, ins, ϵ,
       κ var x : τ @ i ⋅ k -->   k, x ↦ v;; ϵ *)
-  | step_asgn_r (e1 e2 e2' : Expr.e)  (k : kstmt) :
+  | step_asgn_r (e1 e2 e2' : Exp.t)  (k : kstmt) :
       ℵ ϵ, e2 -->  e2' ->
       ℸ cfg, tbls, aa, fns, ins, ϵ,
       κ asgn e1 := e2 @ i ⋅ k -->  κ asgn e1 := e2' @ i ⋅ k, ϵ
-  | step_asgn_l (e1 e1' v2 : Expr.e)  (k : kstmt) :
+  | step_asgn_l (e1 e1' v2 : Exp.t)  (k : kstmt) :
       value v2 ->
       ℶ e1 -->  e1' ->
       ℸ cfg, tbls, aa, fns, ins, ϵ,
       κ asgn e1 := v2 @ i ⋅ k -->  κ asgn e1' := v2 @ i ⋅ k, ϵ
-  | step_asgn (v1 v2 : Expr.e)  (k : kstmt) :
+  | step_asgn (v1 v2 : Exp.t)  (k : kstmt) :
       lvalue v1 ->
       value v2 ->
       let ϵ' := lv_update v1 v2 ϵ in
@@ -190,22 +190,22 @@ Module Step.
       ℸ cfg, tbls, aa, fns, ins, ϵ, EXIT ∫ ϵk ⊗ k -->  EXIT k, (ϵk ≪ ϵ)
   | step_return_void  (k : kstmt) :
       ℸ cfg, tbls, aa, fns, ins, ϵ, κ return None @ i ⋅ k -->  VOID k, ϵ
-  | step_return_fruit (e e' : Expr.e) (τ : Expr.t)  (k : kstmt) :
+  | step_return_fruit (e e' : Exp.t) (τ : Typ.t)  (k : kstmt) :
       ℵ ϵ, e -->  e' ->
            let eo := Some e in
            let eo' := Some e' in
       ℸ cfg, tbls, aa, fns, ins, ϵ,
       κ return eo @ i ⋅ k -->  κ return eo' @ i ⋅ k, ϵ
-  | step_return_value (v : Expr.e) (τ : Expr.t)  (k : kstmt) :
+  | step_return_value (v : Exp.t) (τ : Typ.t)  (k : kstmt) :
       value v ->
       let eo := Some v in
       ℸ cfg, tbls, aa, fns, ins, ϵ,
       κ return eo @ i ⋅ k -->  FRUIT v k, ϵ
-  | step_kreturn_kseq (o : option (Expr.e)) (s : Stmt.s) (k : kstmt) :
+  | step_kreturn_kseq (o : option (Exp.t)) (s : Stmt.s) (k : kstmt) :
       ℸ cfg, tbls, aa, fns, ins, ϵ, RETURN o κ s ⋅ k -->  RETURN o k, ϵ
-  | step_kreturn_kblock (o : option (Expr.e)) (ϵk : eenv) (k : kstmt) :
+  | step_kreturn_kblock (o : option (Exp.t)) (ϵk : eenv) (k : kstmt) :
       ℸ cfg, tbls, aa, fns, ins, ϵ, EXIT ∫ ϵk ⊗ k -->  EXIT k, (ϵk ≪ ϵ)
-  | step_cond (e e' : Expr.e) (s1 s2 : Stmt.s)  (k : kstmt) :
+  | step_cond (e e' : Exp.t) (s1 s2 : Stmt.s)  (k : kstmt) :
       ℵ ϵ, e -->  e' ->
       ℸ cfg, tbls, aa, fns, ins, ϵ,
       κ if e then s1 else s2 @ i ⋅ k -->
@@ -216,9 +216,9 @@ Module Step.
   | step_cond_false (s1 s2 : Stmt.s) (i' i :) (k : kstmt) :
       ℸ cfg, tbls, aa, fns, ins, ϵ,
       κ if FALSE @ i' then s1 else s2 @ i ⋅ k -->  κ s2 ⋅ k, ϵ
-  | step_funcall_in_arg (prefix suffix : Expr.args) (f x : string)
-                        (e e' : Expr.e)
-                        (o : option (Expr.e))
+  | step_funcall_in_arg (prefix suffix : Exp.args) (f x : string)
+                        (e e' : Exp.t)
+                        (o : option (Exp.t))
                          (k : kstmt) :
       F.predfs_data (pred_paramarg value lvalue) prefix ->
       ℵ ϵ, e -->  e' ->
@@ -227,15 +227,15 @@ Module Step.
       ℸ cfg, tbls, aa, fns, ins, ϵ,
       κ funcall f <[]> (args)  into o @ i ⋅ k -->
       κ funcall f <[]> (args') into o @ i ⋅ k, ϵ
-   | step_funcall_lvalue (args : Expr.args) (f : string)
-                         (e e' : Expr.e)  (k : kstmt) :
+   | step_funcall_lvalue (args : Exp.args) (f : string)
+                         (e e' : Exp.t)  (k : kstmt) :
        F.predfs_data (pred_paramarg value lvalue) args ->
        ℶ e -->  e' ->
        ℸ cfg, tbls, aa, fns, ins, ϵ,
        κ let e  := call f <[]> (args) @ i ⋅ k -->
        κ let e' := call f <[]> (args) @ i ⋅ k, ϵ
-   | step_funcall (args : Expr.args) (f : string)
-                  (o : option (Expr.e))
+   | step_funcall (args : Exp.args) (f : string)
+                  (o : option (Exp.t))
                    (k : kstmt)
                   (body : Stmt.s) (fϵ : eenv)
                   (fclosure : fenv) (fins : ienv) :
@@ -247,16 +247,16 @@ Module Step.
        ℸ cfg, tbls, aa, fns, ins, ϵ,
        κ funcall f <[]> (args) into o @ i ⋅ k -->
        κ body ⋅ Λ (arrow, ϵ) k, fϵ'
-   | step_kexit_kcall (ϵk : eenv) (args : Expr.args) (k : kstmt) :
+   | step_kexit_kcall (ϵk : eenv) (args : Exp.args) (k : kstmt) :
        let ϵ' := copy_out args ϵ ϵk in
        let arrow := {|paramargs:=args; rtrns:=None|} in
        ℸ cfg, tbls, aa, fns, ins, ϵ, EXIT Λ (arrow, ϵk) k -->  k, ϵ'
-   | step_void_kcall (ϵk : eenv) (args : Expr.args) (k : kstmt) :
+   | step_void_kcall (ϵk : eenv) (args : Exp.args) (k : kstmt) :
        let ϵ' := copy_out args ϵ ϵk in
        let arrow := {|paramargs:=args; rtrns:=None|} in
        ℸ cfg, tbls, aa, fns, ins, ϵ, VOID Λ (arrow, ϵk) k -->  k, ϵ'
-   | step_fruit_kcall (v lv : Expr.e) (ϵk : eenv)
-                      (args : Expr.args) (k : kstmt) :
+   | step_fruit_kcall (v lv : Exp.t) (ϵk : eenv)
+                      (args : Exp.args) (k : kstmt) :
        let ϵ' := ϵk ▷ copy_out args ϵ ▷ lv_update lv v in
        let arrow := {|paramargs:=args; rtrns:=Some lv|} in
        ℸ cfg, tbls, aa, fns, ins, ϵ, FRUIT v Λ (arrow, ϵk) k -->  k, ϵ'
