coq/lib/P4cub/Transformations/Lifting/LiftSpec.v
@@ -42,20 +42,20 @@ End RelateDeclList.
 Section RelateExprDeclList.
   Polymorphic Universe a.
   Polymorphic Context {A : Type@{a}}.
-  Polymorphic Variable R : list A -> Expr.e -> A -> Prop.
+  Polymorphic Variable R : list A -> Exp.t -> A -> Prop.
   Polymorphic Variable l : list A.
 
-  Polymorphic Hypothesis shift_e_preserves_R : forall as1 as2 as3 a e,
+  Polymorphic Hypothesis shift_exp_preserves_R : forall as1 as2 as3 a e,
       R (as1 ++ as3) e a ->
-      R (as1 ++ as2 ++ as3) (shift_e (Shifter (length as1) (length as2)) e) a.
+      R (as1 ++ as2 ++ as3) (shift_exp (Shifter (length as1) (length as2)) e) a.
 
   Local Hint Constructors relate_decl_list : core.
   
   Polymorphic Lemma relate_decl_list_app : forall es1 es2 as1 as2,
       relate_decl_list R l es1 as1 ->
       relate_decl_list R l es2 as2 ->
-      relate_decl_list R l (shift_list shift_e (Shifter 0 (length es1)) es2 ++ es1) (as2 ++ as1).
-  Proof using A R l shift_e_preserves_R.
+      relate_decl_list R l (shift_list shift_exp (Shifter 0 (length es1)) es2 ++ es1) (as2 ++ as1).
+  Proof using A R l shift_exp_preserves_R.
     intros es1 es2 as1 as2 h1 h2.
     generalize dependent as1.
     generalize dependent es1.
@@ -73,9 +73,9 @@ Section RelateExprDeclList.
   Polymorphic Lemma shift_pairs_relate_snd : forall ess ass,
       Forall2 (relate_decl_list R l) (map snd ess) ass ->
       relate_decl_list R l
-        (concat (map snd (shift_pairs shift_e ess)))
+        (concat (map snd (shift_pairs shift_exp ess)))
         (concat ass).
-  Proof using A R l shift_e_preserves_R.
+  Proof using A R l shift_exp_preserves_R.
     intros ess vss h.
     remember (map snd ess) as sess eqn:hess.
     generalize dependent ess.
@@ -83,8 +83,8 @@ Section RelateExprDeclList.
       unravel in *; auto.
     pose proof IHh ess ltac:(auto) as ih; clear IHh.
     rewrite map_snd_map, map_id.
-    assert (list_sum (map (length (A:=Expr.e)) (map snd ess))
-            = length (concat (map snd (shift_pairs shift_e ess)))) as hlen.
+    assert (list_sum (map (length (A:=Exp.t)) (map snd ess))
+            = length (concat (map snd (shift_pairs shift_exp ess)))) as hlen.
     { unfold list_sum.
       rewrite sublist.length_concat.
       rewrite shift_pairs_inner_length.
@@ -98,8 +98,8 @@ Section RelateExprDeclList.
       Forall2 (relate_decl_list R l) ess vss ->
       Forall2
         (R (concat vss ++ l))
-        (map fst (shift_pairs shift_e (combine es ess))) vs.
-  Proof using A R l shift_e_preserves_R.
+        (map fst (shift_pairs shift_exp (combine es ess))) vs.
+  Proof using A R l shift_exp_preserves_R.
     intros es ess vs vss hl hF3.
     generalize dependent ess.
     induction hF3; intros [| E ess] hl hF2;
@@ -123,7 +123,7 @@ Section RelateExprDeclList.
       reflexivity. }
     rewrite hlen.
     rewrite (relate_decl_list_length _ _ _ _ H3).
-    constructor; auto using shift_e_preserves_R.
+    constructor; auto using shift_exp_preserves_R.
     pose proof IHhF3 _ H1 H5 as ih; clear IHhF3.
     clear dependent v.
     clear dependent E.
@@ -136,13 +136,13 @@ Section RelateExprDeclList.
       assumption.
     - intros n e v he hv.
       rewrite nth_error_map in he.
-      destruct (nth_error (map fst (shift_pairs shift_e (combine us ess))) n)
+      destruct (nth_error (map fst (shift_pairs shift_exp (combine us ess))) n)
         as [se |] eqn:hse;
         cbn in *;
         try discriminate.
       inv he.
       pose proof ih _ _ _ hse hv as h.
-      pose proof shift_e_preserves_R [] t0 _ _ _ h as H;
+      pose proof shift_exp_preserves_R [] t0 _ _ _ h as H;
         cbn in H.
       assumption.
   Qed.
